\documentclass[10pt]{article}
\usepackage[utf8]{inputenc}
\usepackage{amsmath}

% partial derivative as a fraction
\newcommand{\fracpd}[2]{
  \ensuremath{\frac{\partial #1}{\partial #2}}
}

% fraction with parenthesis around it
\newcommand{\pfrac}[2]{
  \ensuremath{ \left( \frac{#1}{#2} \right)}
}



\begin{document}

\section{Model}

  The unscaled model can be written as

  \begin{align*}
    J(k_1, k_2, z_1, z_2, U) &= \max_{c_1, c_2, I_1, I_2, U'} \left[ (1 - \beta_1) c_1^{\rho_1} + \beta_1 \mu(J')^\rho \right]^{\frac{1}{\rho_1}} \\
    \text{subject to }& \left[ (1 - \beta_2) c_2^{\rho_2} + \beta_2 \mu(U')^\rho \right]^{\frac{1}{\rho_2}} \\
    c_1 + c_2 + I_1 + I_2 &= f_1(k_1, z_1) + f_2(k_2, z_2) \\
    k_1' &= \Gamma_1(k_1, I_1) \\
    k_2' &= \Gamma_2(k_2, I_2) \\
  \end{align*}

  where

  \begin{align*}
    f_1(k_1, z_1) &= \left[(1 - \eta_1) k_1^{\nu_1} + \eta_1 z_1^{\nu_1}] \right]^{\frac{1}{\nu_1}} \\
    f_2(k_2, z_2) &= \left[(1 - \eta_2) k_2^{\nu_2} + \eta_2 z_2^{\nu_2}] \right]^{\frac{1}{\nu_2}} \\
    \Gamma_1(k_1, I_1) &= \left[(1 - \delta) k_1^{\gamma_1} + \delta I_1^{\gamma_1} \right]^{\frac{1}{\gamma_1}} \\
    \Gamma_2(k_2, I_2) &= \left[(1 - \delta) k_2^{\gamma_2} + \delta I_2^{\gamma_2} \right]^{\frac{1}{\gamma_2}}
  \end{align*}

  Note: For $\gamma_i = 1$ and $I_i = 0$ that we get $k_{t+1} = (1 - \delta) k_t$ which is the standard rate of depreciation.

  If we then scale the model by $z_1$, we get\footnote{I'm going to use same variable names, but everything in site is scaled by $z_1$}

  \begin{align*}
    J(k_1, k_2, \xi, U) &= \max_{c_1, c_2, I_1, I_2, U'} \left[ (1 - \beta_1) c_1^{\rho_1} + \beta_1 \mu(g' J')^\rho \right]^{\frac{1}{\rho_1}} \\
    \text{subject to }& \left[ (1 - \beta_2) c_2^{\rho_2} + \beta_2 \mu(g' U')^\rho \right]^{\frac{1}{\rho_2}} \\
    c_1 + c_2 + I_1 + I_2 &= f_1(k_1) + f_2(k_2, \xi) \\
    g' k_1' &= \Gamma_1(k_1, I_1) \\
    g' k_2' &= \Gamma_2(k_2, I_2) \\
  \end{align*}


\section{First Order Conditions}

  \begin{align*}
    c_1 &: J^{1 - \rho_1} (1 - \beta_1) c_1^{\rho_1 - 1} + \text{LM on BC} = 0 \\
    c_2 &: U^{1 - \rho_2} (1 - \beta_2) c_2^{\rho_2 - 1} + \text{LM on BC} = 0 \\
    I_1 &: J^{1 - \rho_1} \beta_1 \mu_1(g' J')^{\rho - 1} (...) + \text{...} \\
    I_2 &: U^{1 - \rho_2}
  \end{align*}





\end{document}
